
(a)* Prove all the results (7)-(12) above.

(b) Show that for any events A and B, $P(A) - P(B) ≤ P(A ∩ B^c).$

(c)* Boole's inequality. For any events $$
A_1, A_2, ..., A_n
$$show that
$$
P\left(\bigcup_{r=1}^{n} A_r\right) \leq \sum_{r=1}^{n} P(A_r).
$$

# a

$$
\begin{flalign*}
(7)\quad P(A^c)=1-P(A)&&
\end{flalign*}
$$

## Proof:

A and $A^c$ are disjoint with union $\Omega$; thus  
If $P(A)+P(A^c)=P(\Omega)=1$  
$P(A^c)=1-P(A)$

$$
\begin{flalign*}
(8)\quad P(\emptyset)=0,&&
\end{flalign*}
$$

## Proof:

If $P(A)+P(A^c)=P(\Omega)=1$  
$P(\emptyset)=P(\Omega^c)=1-P(\Omega)=0$.  

$$
\begin{flalign*}
(9)\quad P(A \cup B)=P(A)+P(B)-P(A \cap B),&&
\end{flalign*}
$$

## Proof:

$$
\begin{flalign*}
A \cup B = (A - (A \cap B)) \cup (B - (B \cap A)) \cup (A \cap B) \\
\\
P(A \cup B) = P(A - (A \cap B)) + P(B - (B \cap A)) + (A \cap B)) \\
\\
= P(A) - P(A \cap B) + P(B) - P(B \cap A) + (A \cap B)) \\
\\
= P(A)+P(B)-P(A \cap B)
&&
\end{flalign*}
$$

$$
\begin{flalign*}
(10)\quad P(A) \leq P(B),\text{ if }A \subseteq B,&&
\end{flalign*}
$$

## Proof:

If A$\subseteq$ B then $B=A\cup(B-A)$

$P(B) = P(A) \cup P(B-A)=P(A)+P(B)-P(A)=P(B)$

$$
\begin{flalign*}
(11)\quad P\left(\bigcup_{r=1}^{n} A_r\right)=\sum_{r=1}^{n} P(A_r)-\sum_{r<s} P(A_r \cap A_s)+\cdots+(-1)^{n+1}P\left(\bigcap_{r=1}^{n} A_r\right),&&
\end{flalign*}
$$

## Proof:

### **Inclusion-Exclusion Principle**
For any finite collection of events $A_1, A_2, \dots, A_n$, the probability of their union is given by:

$$
\begin{flalign*}
P\left(\bigcup_{r=1}^{n} A_r\right) = \sum_{r=1}^{n} P(A_r) - \sum_{r < s} P(A_r \cap A_s) + \cdots + (-1)^{n+1} P\left(\bigcap_{r=1}^{n} A_r\right).&&
\end{flalign*}
$$
#### **Base Case (\( n = 1 \))**

For \( n = 1 \), the formula reduces to:

$P(A_1) = P(A_1)$

which is trivially true.

#### **Inductive Step**

Assume the formula holds for \( n = k \), i.e.,

$$
P\left(\bigcup_{r=1}^{k} A_r\right) = \sum_{i=1}^{k} P(A_i) - \sum_{1 \leq i < j \leq k} P(A_i \cap A_j) + \cdots + (-1)^{k+1} P\left(\bigcap_{r=1}^{k} A_r\right).
$$

We must show that it holds for \( n = k + 1 \).

Consider the union of \( k + 1 \) events:

$$
P\left(\bigcup_{r=1}^{k+1} A_r\right) = P\left(\left(\bigcup_{r=1}^{k} A_r\right) \cup A_{k+1}\right).
$$

Using the **inclusion-exclusion principle for two events**:

$$
P(B \cup C) = P(B) + P(C) - P(B \cap C),
$$

where $B = \bigcup_{r=1}^{k} A_r$ and $C = A_{k+1}$, we get:

$$
P\left(\bigcup_{r=1}^{k+1} A_r\right) = P\left(\bigcup_{r=1}^{k} A_r\right) + P(A_{k+1}) - P\left(\bigcup_{r=1}^{k} (A_r \cap A_{k+1})\right).
$$

Now, apply the **inductive hypothesis** to $P\left(\bigcup_{r=1}^{k} A_r\right)$ and $P\left(\bigcup_{r=1}^{k} (A_r \cap A_{k+1})\right)$:

$$
P\left(\bigcup_{r=1}^{k} A_r\right) = \sum_{i=1}^{k} P(A_i) - \sum_{1 \leq i < j \leq k} P(A_i \cap A_j) + \cdots + (-1)^{k+1} P\left(\bigcap_{r=1}^{k} A_r\right)
$$

$$
P\left(\bigcup_{r=1}^{k} (A_r \cap A_{k+1})\right) = \sum_{i=1}^{k} P(A_i \cap A_{k+1}) - \sum_{1 \leq i < j \leq k} P(A_i \cap A_j \cap A_{k+1}) + \cdots + (-1)^{k+1} P\left(\bigcap_{r=1}^{k+1} A_r\right).
$$
Substituting these into the previous equation and collecting terms, we obtain:
$$
P\left(\bigcup_{r=1}^{k+1} A_r\right) = \sum_{i=1}^{k+1} P(A_i) - \sum_{1 \leq i < j \leq k+1} P(A_i \cap A_j) + \cdots + (-1)^{k+2} P\left(\bigcap_{r=1}^{k+1} A_r\right).
$$
Thus, the formula holds for $n = k + 1$.

By the principle of mathematical induction, the inclusion-exclusion principle holds for all $n \geq 1$. $\triangle$

$$
\begin{flalign*}
(12)\quad\text{if }\lim_{n \to \infty} A_n=A,\text{ then }\lim_{n \to \infty} P(A_n)=P(A).&&
\end{flalign*}
$$

## [Proof:](https://www.youtube.com/watch?v=qZoOFY78lzw)

If $(B_n)$ is an increasing sequence of events, $B_1\subseteq B_2\subseteq\dots\subseteq B=\lim_{n\to\infty}B_n$, then by (5),  
$$P(B)=P(B_1)+\lim_{n\to\infty}\sum_{r=1}^{n-1}[P(B_{r+1})-P(B_r)]=\lim_{n\to\infty}P(B_n).$$  
The same is true for a decreasing sequence ($D_n$). Let $D_n=\bigcup_{m=n}^\infty A_m$, and $B_n=\bigcap_{m=n}^\infty A_m$. Then, $D_n$ and $B_n$ are decreasing and increasing, respectively, with limit A. The result follows. 

# b

$$
P(A) − P(B) ≤ P(A ∩ B)
$$
$$
P(A \cap B) = P(A) + P(B) - P(A \cup B)
$$
$$
P(A) − P(B) ≤ P(A) + P(B) - P(A \cup B)
$$
$$
P(A \cup B) \leq 2P(B)
$$
Which is not always true

# c

$$
P\left(\bigcup_{r=1}^{n} A_r\right) \leq \sum_{r=1}^{n} P(A_r).
$$
## [Proof:](https://www.youtube.com/watch?v=PECnoM5hUIo)

Use induction and (1.1.9)